RocqOfRust/revm/revm_interpreter/instructions/simulate/host/selfdestruct.v
@@ -1,16 +1,25 @@
 Require Import simulate.RocqOfRust.
 Require Import alloy_primitives.links.aliases.
+Require Import core.links.result.
 Require Import core.links.array.
 Require Import revm.revm_context_interface.links.host.
 Require Import revm.revm_context_interface.links.journaled_state.
 Require Import revm.revm_context_interface.simulate.host.
+Require Import revm.revm_interpreter.gas.simulate.calc.
+Require Import revm.revm_interpreter.gas.simulate.constants.
 Require Import revm.revm_interpreter.instructions.links.host.selfdestruct.
 Require Import revm.revm_interpreter.instructions.simulate.macros.
 Require Import revm.revm_interpreter.instructions.simulate.utility.
+Require Import revm.revm_interpreter.links.gas.
 Require Import revm.revm_interpreter.links.interpreter.
+Require Import revm.revm_interpreter.links.instruction_context.
 Require Import revm.revm_interpreter.links.instruction_result.
 Require Import revm.revm_interpreter.links.interpreter_types.
+Require Import revm.revm_interpreter.simulate.gas.
+Require Import revm.revm_interpreter.simulate.interpreter.
 Require Import revm.revm_interpreter.simulate.interpreter_types.
+Require Import revm.revm_primitives.links.hardfork.
+Require Import revm.revm_primitives.simulate.hardfork.
 
 Definition selfdestruct
     {WIRE H : Set} `{Link WIRE} `{Link H}
@@ -21,27 +30,46 @@ Definition selfdestruct
     (interpreter : Interpreter.t WIRE WIRE_types)
     (host : H) :
     Interpreter.t WIRE WIRE_types * H :=
-  let set_result
-      (interpreter : Interpreter.t WIRE WIRE_types)
-      (result : InstructionResult.t) :=
-    let control :=
-      IInterpreterTypes.(InterpreterTypes.LoopControl_for_Control).(LoopControl.set_instruction_result)
-        interpreter.(Interpreter.control)
-        result in
-    interpreter <| Interpreter.control := control |> in
+  require_non_staticcall_macro interpreter
+    (fun interpreter => (interpreter, host)) (fun interpreter =>
   popn_macro interpreter 1 (fun interpreter => (interpreter, host)) (fun arr interpreter =>
     let '⟬ target_u256 ⟭ := arr.(array.value) in
     let target := Impl_IntoAddress_for_U256.into_address target_u256 in
+    let spec_id :=
+      IInterpreterTypes.(InterpreterTypes.RuntimeFlag_for_RuntimeFlag).(RuntimeFlag.spec_id)
+        interpreter.(Interpreter.runtime_flag) in
+    gas_macro interpreter
+      (calc.static_selfdestruct_cost spec_id)
+      (fun interpreter => (interpreter, host)) (fun interpreter =>
+    let skip_cold_load :=
+      i[interpreter.(Interpreter.gas).(Gas.remaining)] <?
+        i[calc.selfdestruct_cold_beneficiary_cost spec_id] in
     let address :=
       IInterpreterTypes.(InterpreterTypes.InputsTrait_for_Input).(InputTraits.target_address)
         interpreter.(Interpreter.input) in
-    let '(result, host) := IHost.(Host.selfdestruct) host address target in
+    let '(result, host) := IHost.(Host.selfdestruct) host address target skip_cold_load in
     match result with
-    | Some _ =>
-      (set_result interpreter instruction_result.InstructionResult.SelfDestruct, host)
-    | None =>
-      (set_result interpreter instruction_result.InstructionResult.FatalExternalError, host)
-    end
+    | Result.Ok state_load =>
+      let state_load_ref : '& (StateLoad.t SelfDestructResult.t) :=
+        Ref.immediate Pointer.Kind.Ref state_load in
+      gas_macro interpreter
+        (calc.dyn_selfdestruct_cost spec_id state_load_ref)
+        (fun interpreter => (interpreter, host)) (fun interpreter =>
+      let is_london := Impl_SpecId.is_enabled_in spec_id SpecId.LONDON in
+      let should_refund :=
+        negb is_london && negb state_load.(StateLoad.data).(SelfDestructResult.previously_destroyed) in
+      let interpreter :=
+        if should_refund then
+          let gas := Impl_Gas.record_refund interpreter.(Interpreter.gas) constants.SELFDESTRUCT_REFUND in
+          interpreter <| Interpreter.gas := gas |>
+        else
+          interpreter in
+      (halt interpreter instruction_result.InstructionResult.SelfDestruct, host))
+    | Result.Err LoadError.ColdLoadSkipped =>
+      (halt_oog interpreter, host)
+    | Result.Err LoadError.DBError =>
+      (halt_fatal interpreter, host)
+    end))
   ).
 
 Lemma selfdestruct_eq
@@ -59,10 +87,14 @@ Lemma selfdestruct_eq
     (host : H) :
   let ref_interpreter := make_ref 0 in
   let ref_host := make_ref (A := H) 1 in
+  let context := {|
+    instruction_context.InstructionContext.interpreter := ref_interpreter;
+    instruction_context.InstructionContext.host := ref_host;
+  |} in
   let result := selfdestruct interpreter host in
   {{
     SimulateM.eval_f
-      (run_selfdestruct run_InterpreterTypes_for_WIRE run_Host_for_H ref_interpreter ref_host)
+      (run_selfdestruct run_InterpreterTypes_for_WIRE run_Host_for_H context)
       [interpreter; host]%stack 🌲
     (
       Output.Success tt,
